progress in reduction and execution lemmas needed for proving exec reducibility

txn-data-consistency/EP+_Reduction.thy
@@ -4,32 +4,27 @@ theory "EP+_Reduction"
   imports "EP+" Reductions
 begin
 
-datatype movt = Lm | Rm
+datatype movt = Lm | Rm | Out
 
-definition mover_type :: "'v ev list \<Rightarrow> nat \<Rightarrow> movt" where
-  "mover_type tr i \<equiv> (let e = tr ! i in
-    (if ev_cl e = ev_cl (hd tr) then Rm else
-     (if ev_cl e = ev_cl (last tr) then Lm else
-      (if (\<exists>j l. l < j \<and> j \<le> i \<and>
-            ev_cl (tr ! j) = ev_cl (tr ! i) \<and>
-            ev_cl (tr ! l) = ev_cl (hd tr) \<and>
-            ev_key (tr ! l) = ev_key (tr ! j) \<and> ev_key (tr ! j) \<noteq> None) then Rm else Lm)))
-  )"
+definition mover_type :: "'v ev list \<Rightarrow> nat \<Rightarrow> nat \<Rightarrow> nat \<Rightarrow> movt" where
+  "mover_type tr i j k \<equiv> (if j \<le> i \<and> i \<le> k then
+   (let e = tr ! i in
+    (if ev_cl e = ev_cl (tr ! j) then Rm else
+     (if ev_cl e = ev_cl (tr ! k) then Lm else
+      (if (\<exists>l m. l < m \<and> m \<le> i \<and>
+            ev_cl (tr ! m) = ev_cl (tr ! i) \<and>
+            ev_cl (tr ! l) = ev_cl (tr ! j) \<and>
+            ev_key (tr ! l) = ev_key (tr ! m) \<and> ev_key (tr ! m) \<noteq> None) then Rm else Lm)))
+  ) else Out)"
 
 definition Lm_dist_left where
-  "Lm_dist_left i j tr \<equiv>
-    Sum {d | d. mover_type (take (Suc (j - i)) (drop i tr)) d = Lm}"
-
-definition left_most_pair :: "'v ev list \<Rightarrow> (nat \<times> nat)" where
-  "left_most_pair tr \<equiv> (ARG_MIN (fst) (i, j). (i, j) \<in> inverted_pairs ev_ects tr \<and>
-    (\<forall>l. i < l \<and> l < j \<longrightarrow>
-      (i, l) \<notin> inverted_pairs ev_ects tr \<and>
-      (l, j) \<notin> inverted_pairs ev_ects tr))"
+  "Lm_dist_left tr j k \<equiv>
+    Sum {i - j | i. mover_type tr i j k = Lm}"
 
 definition lmp_dist_left :: "('v ev, ('v, 'm) global_conf_scheme) exec_frag \<Rightarrow> nat" where
   "lmp_dist_left ef \<equiv>
-    let (i, j) = left_most_pair (trace_of_efrag ef) in
-      Lm_dist_left i j (trace_of_efrag ef)"
+    let (j, k) = left_most_adj_pair ev_ects (trace_of_efrag ef) in
+      Lm_dist_left (trace_of_efrag ef) j k"
 
 definition measure_R :: "('v ev, ('v, 'm) global_conf_scheme) exec_frag rel" where
   "measure_R \<equiv> measures [card o inverted_pairs ev_ects o trace_of_efrag, lmp_dist_left]"
@@ -37,15 +32,47 @@ definition measure_R :: "('v ev, ('v, 'm) global_conf_scheme) exec_frag rel" whe
 lemma wf_measure_R: "wf measure_R"
   by (auto simp add: measure_R_def)
 
+lemma mover_type_left_end:
+  "j < k \<Longrightarrow> mover_type tr j j k = Rm"
+  by (auto simp add: mover_type_def)
+
+lemma mover_type_right_end:
+  "j < k \<Longrightarrow> ev_cl (tr ! j) \<noteq> ev_cl (tr ! k) \<Longrightarrow> mover_type tr k j k = Lm"
+  by (auto simp add: mover_type_def)
+
+lemma inverted_pair_not_same_cl:
+  "(j, k) \<in> inverted_pairs ev_ects tr \<Longrightarrow> ev_cl (tr ! j) \<noteq> ev_cl (tr ! k)"
+  apply (auto simp add: inverted_pairs_def ects_def) 
+  oops
+
 lemma reducible_exec_frag:
   assumes
     \<open>valid_exec_frag tps ef\<close>
     \<open>ef \<notin> Good_wrt ev_ects\<close>
   shows
     \<open>\<exists>ef'. tps: ef \<rhd> ef' \<and> (ef' \<in> Good_wrt ev_ects \<or> (ef', ef) \<in> measure_R)\<close>
-  using assms reduce_frag_left_commute
+proof - 
+  have "\<exists>j k. adj_inv_pair ev_ects (trace_of_efrag ef) j k" using assms(2)
+    by (simp add: adj_inv_exists_not_Good_ex)
+  then have e: "\<exists>j k. is_arg_min (fst) (\<lambda>(i, j). adj_inv_pair ev_ects (trace_of_efrag ef) i j) (j, k)"
+    by (smt (verit, del_insts) arg_min_natI case_prodE case_prodI is_arg_min_arg_min_nat)
+  then obtain j k where *: "(j, k) = left_most_adj_pair ev_ects (trace_of_efrag ef)"
+    by (metis nat_gcd.cases)
+  then have **: "adj_inv_pair ev_ects (trace_of_efrag ef) j k"
+    using e unfolding left_most_adj_pair_def
+    by (smt (verit, best) arg_min_natI case_prodD is_arg_min_def)
+  then obtain i where
+    "j \<le> i \<and> Suc i \<le> k"
+    "mover_type (trace_of_efrag ef) i j k = Rm"
+    "mover_type (trace_of_efrag ef) (Suc i) j k = Lm" sorry (* needs showing j, k don't have the same cl *)
+  then show ?thesis using assms * **
+      valid_exec_decompose[of tps ef i]
+      reduce_frag_left_commute[of tps ef "ef_first ef" "take i (ef_list ef)" "states_of_efrag ef ! i"
+        "trace_of_efrag ef ! i" "states_of_efrag ef ! Suc i" "trace_of_efrag ef ! (Suc i)"
+        "states_of_efrag ef ! Suc (Suc i)" "drop (Suc (Suc i)) (ef_list ef)" "ef_last ef"]
   apply (auto simp add: Good_wrt_def)
-  sorry
+    sorry
+qed
 
 lemma reducible_to_Good_wrt_f_exec_frag: 
   "reducible tps (Good_wrt ev_ects)"
